Flapjack/Test/Allocator.lean
@@ -94,4 +94,21 @@ example [OfNat α 1] :
     loopToWordProg, wordCompileExp, wordFindVar, wordMapVars, lookupNatInfo,
     List.eraseDups, List.eraseDupsBy, List.eraseDupsBy.loop]
 
+example [OfNat α 1] :
+    pipelineWordFunctionsAllocatedWithAnalysisAndColour
+      [(0, [0], (.assign 1 (.var 0) : LoopProg α))] =
+      some [(0, [2], (.assign 3 (.var 2) : WordProg α))] := by
+  simp [pipelineWordFunctionsAllocatedWithAnalysisAndColour,
+    wordAllocateProgramWithSlotsAndColour, wordAllocateContextWithClashes,
+    wordAllocateVarsWithClashes, wordGreedyColour, wordColourCandidates,
+    wordFirstAvailable, wordPreferredRegister, wordAllocatableRegisters,
+    wordNeighbours, wordUsedRegisters, wordRegisterIsAllocatable,
+    wordColouringUsesAllocatable, wordColouringRespectsClashes,
+    wordProgClashAnalysis, wordProgVariables, wordProgReadVars,
+    wordProgWriteVars, wordProgLiveBefore, wordProgAtomicClashes,
+    wordClashPairs, wordExpReadVars, loopAccVars, loopVarsOfExp,
+    loopInsertAll, loopInsert, loopToWordProg, wordCompileExp, wordFindVar,
+    wordApplyColour, wordApplyColourExp, wordMapVars, lookupNatInfo,
+    List.eraseDups, List.eraseDupsBy, List.eraseDupsBy.loop]
+
 end Flapjack
